Velvet/Core.lean
@@ -7,6 +7,7 @@ public import Velvet.Core.Specs
 public import Velvet.Core.Loop
 public import Velvet.Core.Partial
 public import Velvet.Core.VCGen
+public import Velvet.Core.NonDet
 
 open scoped GhostSyntax Std.WP Lean.Order
-open Std.WP Named Loop Specs WPPartial
+open Std.WP Named Loop Specs WPPartial NonDetT
