Velvet/Examples.lean
@@ -24,3 +24,4 @@ public import Velvet.Examples.HypNaming
 public import Velvet.Examples.LiftingExamples
 public import Velvet.Examples.VelvetAndIntrinsicVerification
 public import Velvet.Examples.SimplestSort
+public import Velvet.Examples.NonDet
